rocq/theories/TypeSystem/EnvTypingSoundness.v
@@ -1,6 +1,6 @@
 From Facet.TypeSystem Require Import Lifetime Types Syntax PathState Program
   TypingRules TypeChecker EnvStructuralRules EnvSoundnessFacts CheckerSoundness.
-From Stdlib Require Import List String Bool Lia.
+From Stdlib Require Import List String Bool Lia PeanoNat.
 Import ListNotations.
 
 (* ------------------------------------------------------------------ *)
@@ -41,7 +41,6 @@ Proof.
     + destruct (IH T b Hlookup) as [st0 [Hstate Hconsumed]].
       exists st0. simpl. rewrite Hname. split; assumption.
 Qed.
-
 Fixpoint call_expr (e : expr) : bool :=
   match e with
   | EUnit => true
@@ -150,6 +149,138 @@ Proof.
         -- right. exact Hin.
         -- exact Hinfer0.
       * exact Hcheck.
+Qed.
+
+Fixpoint struct_expr (e : expr) : bool :=
+  match e with
+  | EUnit => true
+  | ELit _ => true
+  | EVar _ => true
+  | EFn _ => true
+  | EPlace _ => true
+  | ELet _ _ _ e1 e2 => struct_expr e1 && struct_expr e2
+  | ELetInfer _ _ e1 e2 => struct_expr e1 && struct_expr e2
+  | ECall _ args => forallb struct_expr args
+  | ECallExpr callee args => struct_expr callee && forallb struct_expr args
+  | EStruct _ _ _ fields => forallb (fun '(_, e_field) => struct_expr e_field) fields
+  | EReplace _ e_new => struct_expr e_new
+  | EAssign _ e_new => struct_expr e_new
+  | EBorrow _ _ => true
+  | EDeref e1 => struct_expr e1
+  | EDrop e1 => struct_expr e1
+  | EIf e1 e2 e3 => struct_expr e1 && struct_expr e2 && struct_expr e3
+  end.
+
+Definition struct_exprs (args : list expr) : bool := forallb struct_expr args.
+
+Lemma struct_exprs_in_true :
+  forall args e,
+    struct_exprs args = true ->
+    In e args ->
+    struct_expr e = true.
+Proof.
+  unfold struct_exprs.
+  intros args e Hargs Hin.
+  rewrite forallb_forall in Hargs.
+  apply Hargs. exact Hin.
+Qed.
+
+Lemma lookup_field_b_struct_expr_true :
+  forall fields name e,
+    forallb (fun '(_, e_field) => struct_expr e_field) fields = true ->
+    lookup_field_b name fields = Some e ->
+    struct_expr e = true.
+Proof.
+  induction fields as [|[fname efield] rest IH]; intros name e Hfields Hlookup; simpl in *.
+  - discriminate.
+  - apply andb_true_iff in Hfields as [Hhead Htail].
+    destruct (String.eqb name fname) eqn:Hname.
+    + inversion Hlookup; subst. exact Hhead.
+    + eapply IH; eassumption.
+Qed.
+
+Fixpoint infer_env_fields_collect fuel env Ω n lts args
+    (Σ : sctx) (fields : list (string * expr)) (defs : list field_def)
+    : infer_result sctx :=
+  match defs with
+  | [] => infer_ok Σ
+  | f :: rest =>
+      match lookup_field_b (field_name f) fields with
+      | None => infer_err (ErrMissingField (field_name f))
+      | Some e_field =>
+          match infer_core_env_state_fuel fuel env Ω n Σ e_field with
+          | infer_err err => infer_err err
+          | infer_ok (T_field, Σ1) =>
+              let T_expected := instantiate_struct_field_ty lts args f in
+              if ty_compatible_b Ω T_field T_expected
+              then infer_env_fields_collect fuel env Ω n lts args Σ1 fields rest
+              else infer_err (compatible_error T_field T_expected)
+          end
+      end
+  end.
+
+Lemma infer_env_fields_collect_eq :
+  forall fuel env Ω n lts args fields defs Σ,
+    (fix go (Σ0 : sctx) (defs0 : list field_def) : infer_result sctx :=
+       match defs0 with
+       | [] => infer_ok Σ0
+       | f :: rest =>
+           match lookup_field_b (field_name f) fields with
+           | None => infer_err (ErrMissingField (field_name f))
+           | Some e_field =>
+               match infer_core_env_state_fuel fuel env Ω n Σ0 e_field with
+               | infer_err err => infer_err err
+               | infer_ok (T_field, Σ1) =>
+                   let T_expected := instantiate_struct_field_ty lts args f in
+                   if ty_compatible_b Ω T_field T_expected
+                   then go Σ1 rest
+                   else infer_err (compatible_error T_field T_expected)
+               end
+           end
+       end) Σ defs =
+    infer_env_fields_collect fuel env Ω n lts args Σ fields defs.
+Proof.
+  intros fuel env Ω n lts args fields defs.
+  induction defs as [|f rest IH]; intros Σ; simpl.
+  - reflexivity.
+  - destruct (lookup_field_b (field_name f) fields) as [e_field |] eqn:Hlookup;
+      try reflexivity.
+    destruct (infer_core_env_state_fuel fuel env Ω n Σ e_field) as [[T_field Σ1] | err]
+      eqn:Hfield; try reflexivity.
+    destruct (ty_compatible_b Ω T_field (instantiate_struct_field_ty lts args f));
+      [rewrite IH |]; reflexivity.
+Qed.
+
+Lemma infer_env_fields_collect_sound :
+  forall fuel env Ω n lts args Σ fields defs Σ',
+    forallb (fun '(_, e_field) => struct_expr e_field) fields = true ->
+    infer_env_fields_collect fuel env Ω n lts args Σ fields defs = infer_ok Σ' ->
+    (forall Σ0 e T Σ1,
+        struct_expr e = true ->
+        infer_core_env_state_fuel fuel env Ω n Σ0 e = infer_ok (T, Σ1) ->
+        typed_env_structural env Ω n Σ0 e T Σ1) ->
+    typed_fields_env_structural env Ω n lts args Σ fields defs Σ'.
+Proof.
+  intros fuel env Ω n lts args Σ fields defs.
+  revert Σ.
+  induction defs as [|f rest IH]; intros Σ Σ' Hfields Hcollect Hexpr; simpl in Hcollect.
+  - inversion Hcollect; subst. constructor.
+  - destruct (lookup_field_b (field_name f) fields) as [e_field |] eqn:Hlookup;
+      try discriminate.
+    destruct (infer_core_env_state_fuel fuel env Ω n Σ e_field) as [[T_field Σ1] | err]
+      eqn:Hfield; try discriminate.
+    destruct (ty_compatible_b Ω T_field (instantiate_struct_field_ty lts args f))
+      eqn:Hcompat; try discriminate.
+    eapply TESFields_Cons.
+    + exact Hlookup.
+    + eapply Hexpr.
+      * eapply lookup_field_b_struct_expr_true; eassumption.
+      * exact Hfield.
+    + exact Hcompat.
+    + eapply IH.
+      * exact Hfields.
+      * exact Hcollect.
+      * exact Hexpr.
 Qed.
 
 Lemma sctx_path_available_success :
@@ -289,6 +420,23 @@ Proof.
       * exact Hstruct.
       * exact Hfield.
       * simpl. rewrite Hbase_path. reflexivity.
+Qed.
+
+Lemma place_under_unique_ref_b_sound :
+  forall env Σ p,
+    place_under_unique_ref_b env Σ p = true ->
+    place_under_unique_ref_structural env Σ p.
+Proof.
+  intros env Σ p.
+  induction p as [x | p IH | p IH field]; intros Hunique; simpl in Hunique.
+  - discriminate.
+  - destruct (infer_place_sctx env Σ p) as [Tp | err] eqn:Hplace; try discriminate.
+    destruct Tp as [u c]; simpl in Hunique.
+    destruct c; try discriminate.
+    destruct r; try discriminate.
+    eapply PUURS_Deref.
+    eapply infer_place_sctx_structural_sound. exact Hplace.
+  - apply PUURS_Field. apply IH. exact Hunique.
 Qed.
 
 Theorem infer_core_env_state_fuel_basic_structural_sound :
@@ -606,6 +754,298 @@ Proof.
       * apply ty_core_eqb_true. exact Hbool.
       * eapply IH; [exact Hcall2 | exact He2].
       * eapply IH; [exact Hcall3 | exact He3].
+      * apply ty_core_eqb_true. exact Hcore.
+      * exact Hmerge.
+Qed.
+
+Theorem infer_core_env_state_fuel_struct_structural_sound :
+  forall fuel env Ω n Σ e T Σ',
+    struct_expr e = true ->
+    infer_core_env_state_fuel fuel env Ω n Σ e = infer_ok (T, Σ') ->
+    typed_env_structural env Ω n Σ e T Σ'.
+Proof.
+  induction fuel as [| fuel' IH]; intros env Ω n Σ e T Σ' Hstruct Hinfer.
+  - simpl in Hinfer. discriminate.
+  - destruct e; simpl in Hstruct; simpl in Hinfer; try discriminate.
+    + inversion Hinfer; subst. constructor.
+    + destruct l; inversion Hinfer; subst; constructor.
+    + destruct (sctx_lookup i Σ) as [[Tvar st] |] eqn:Hlookup; try discriminate.
+      destruct (binding_available_b st []) eqn:Havailable; try discriminate.
+      destruct (consume_place_value env Σ (PVar i) Tvar) as [Σ0 | err] eqn:Hconsume;
+        try discriminate.
+      unfold consume_place_value in Hconsume.
+      destruct (usage_eqb (ty_usage Tvar) UUnrestricted) eqn:Husage.
+      * inversion Hconsume; subst. inversion Hinfer; subst.
+        apply TES_Var_Copy.
+        -- apply TPES_Var with (st := st); assumption.
+        -- apply usage_eqb_true. exact Husage.
+      * simpl in Hconsume.
+        destruct (sctx_consume_path Σ i []) as [Σc | err] eqn:Hconsume_path;
+          try discriminate.
+        inversion Hconsume; subst. inversion Hinfer; subst.
+        eapply TES_Var_Move.
+        -- apply TPES_Var with (st := st); assumption.
+        -- intro Hu. rewrite Hu in Husage. simpl in Husage. discriminate.
+        -- exact Hconsume_path.
+    + apply andb_true_iff in Hstruct as [Hstruct1 Hstruct2].
+      destruct (infer_core_env_state_fuel fuel' env Ω n Σ e1) as [[T1 Σ1] | err1]
+        eqn:He1; try discriminate.
+      destruct (ty_compatible_b Ω T1 t) eqn:Hcompat; try discriminate.
+      destruct (infer_core_env_state_fuel fuel' env Ω n (sctx_add i t m Σ1) e2)
+        as [[T2 Σ2] | err2] eqn:He2; try discriminate.
+      destruct (sctx_check_ok i t Σ2) eqn:Hcheck; try discriminate.
+      inversion Hinfer; subst.
+      eapply TES_Let.
+      * eapply IH; [exact Hstruct1 | exact He1].
+      * exact Hcompat.
+      * eapply IH; [exact Hstruct2 | exact He2].
+      * exact Hcheck.
+    + apply andb_true_iff in Hstruct as [Hstruct1 Hstruct2].
+      destruct (infer_core_env_state_fuel fuel' env Ω n Σ e1) as [[T1 Σ1] | err1]
+        eqn:He1; try discriminate.
+      destruct (infer_core_env_state_fuel fuel' env Ω n (sctx_add i T1 m Σ1) e2)
+        as [[T2 Σ2] | err2] eqn:He2; try discriminate.
+      destruct (sctx_check_ok i T1 Σ2) eqn:Hcheck; try discriminate.
+      inversion Hinfer; subst.
+      eapply TES_LetInfer.
+      * eapply IH; [exact Hstruct1 | exact He1].
+      * eapply IH; [exact Hstruct2 | exact He2].
+      * exact Hcheck.
+    + destruct (lookup_fn_b i (env_fns env)) as [fdef |] eqn:Hlookup; try discriminate.
+      inversion Hinfer; subst.
+      destruct (lookup_fn_b_sound i (env_fns env) fdef Hlookup) as [Hin Hname].
+      eapply TES_Fn; eassumption.
+    + destruct (infer_place_sctx env Σ p) as [Tp | err] eqn:Hplace; try discriminate.
+      destruct (consume_place_value env Σ p Tp) as [Σ0 | err] eqn:Hconsume;
+        try discriminate.
+      unfold consume_place_value in Hconsume.
+      destruct (usage_eqb (ty_usage Tp) UUnrestricted) eqn:Husage.
+      * inversion Hconsume; subst. inversion Hinfer; subst.
+        apply TES_Place_Copy.
+        -- eapply infer_place_sctx_structural_sound. exact Hplace.
+        -- apply usage_eqb_true. exact Husage.
+      * destruct (place_path p) as [[x path] |] eqn:Hpath; try discriminate.
+        destruct (sctx_consume_path Σ x path) as [Σc | err] eqn:Hconsume_path;
+          try discriminate.
+        inversion Hconsume; subst. inversion Hinfer; subst.
+        eapply TES_Place_Move.
+        -- eapply infer_place_sctx_structural_sound. exact Hplace.
+        -- intro Hu. rewrite Hu in Husage. simpl in Husage. discriminate.
+        -- exact Hpath.
+        -- exact Hconsume_path.
+    + destruct (lookup_fn_b i (env_fns env)) as [fdef |] eqn:Hlookup; try discriminate.
+      rewrite infer_env_args_collect_eq in Hinfer.
+      destruct (infer_env_args_collect fuel' env Ω n Σ l) as [[arg_tys Σargs] | err]
+        eqn:Hcollect; try discriminate.
+      destruct (build_sigma (fn_lifetimes fdef) (repeat None (fn_lifetimes fdef))
+          arg_tys (fn_params fdef)) as [σ_acc |] eqn:Hbuild; try discriminate.
+      remember (apply_lt_params (finalize_subst σ_acc) (fn_params fdef)) as ps_subst.
+      destruct (check_args Ω arg_tys ps_subst) as [err |] eqn:Hcheck; try discriminate.
+      destruct (forallb (wf_lifetime_b (mk_region_ctx n)) (finalize_subst σ_acc)) eqn:Hwf;
+        try discriminate.
+      remember (apply_lt_outlives (finalize_subst σ_acc) (fn_outlives fdef)) as Ω_subst.
+      destruct (outlives_constraints_hold_b Ω Ω_subst) eqn:Hout; try discriminate.
+      inversion Hinfer; subst.
+      destruct (lookup_fn_b_sound i (env_fns env) fdef Hlookup) as [Hin Hname].
+      eapply TES_Call with (fdef := fdef) (σ := finalize_subst σ_acc).
+      * exact Hin.
+      * exact Hname.
+      * eapply infer_env_args_collect_sound.
+        -- exact Hcollect.
+        -- intros Σ0 e0 T0 Σ1 Hin_arg Hinfer_arg.
+           eapply IH.
+           ++ eapply struct_exprs_in_true; eassumption.
+           ++ exact Hinfer_arg.
+        -- exact Hcheck.
+      * apply env_outlives_constraints_hold_b_sound. exact Hout.
+    + apply andb_true_iff in Hstruct as [Hcallee Hargs].
+      destruct (infer_core_env_state_fuel fuel' env Ω n Σ e) as [[Tcallee Σc] | err]
+        eqn:Hcallee_infer; try discriminate.
+      rewrite infer_env_args_collect_eq in Hinfer.
+      destruct (infer_env_args_collect fuel' env Ω n Σc l) as [[arg_tys Σargs] | err]
+        eqn:Hcollect; try discriminate.
+      destruct Tcallee as [u c]; simpl in *.
+      destruct c; try discriminate.
+      * destruct (check_arg_tys Ω arg_tys l0) as [err |] eqn:Hcheck; try discriminate.
+        inversion Hinfer; subst.
+        eapply TES_CallExpr_Fn.
+        -- eapply IH; [exact Hcallee | exact Hcallee_infer].
+        -- eapply infer_env_args_collect_sound.
+           ++ exact Hcollect.
+           ++ intros Σ0 e0 T0 Σ1 Hin_arg Hinfer_arg.
+              eapply IH.
+              ** eapply struct_exprs_in_true; eassumption.
+              ** exact Hinfer_arg.
+           ++ rewrite <- check_arg_tys_params_of_tys. exact Hcheck.
+      * destruct (ty_core t) eqn:Hbody; try discriminate.
+        destruct (build_bound_sigma (repeat None n0) arg_tys l0) as [σ |] eqn:Hbuild;
+          try discriminate.
+        destruct (check_arg_tys Ω arg_tys (map (open_bound_ty σ) l0)) as [err |] eqn:Hcheck;
+          try discriminate.
+        destruct (contains_lbound_ty (open_bound_ty σ t0) ||
+            contains_lbound_outlives (open_bound_outlives σ o)) eqn:Hleak;
+          try discriminate.
+        destruct (outlives_constraints_hold_b Ω (open_bound_outlives σ o)) eqn:Hout;
+          try discriminate.
+        inversion Hinfer; subst.
+        apply opened_call_no_lbound_sound in Hleak as [Hret Hbounds].
+        eapply TES_CallExpr_Forall with (σ := σ) (param_tys := l0).
+        -- eapply IH; [exact Hcallee | exact Hcallee_infer].
+        -- exact Hbody.
+        -- eapply infer_env_args_collect_sound.
+           ++ exact Hcollect.
+           ++ intros Σ0 e0 T0 Σ1 Hin_arg Hinfer_arg.
+              eapply IH.
+              ** eapply struct_exprs_in_true; eassumption.
+              ** exact Hinfer_arg.
+           ++ rewrite <- check_arg_tys_params_of_tys. exact Hcheck.
+        -- exact Hret.
+        -- exact Hbounds.
+        -- apply env_outlives_constraints_hold_b_sound. exact Hout.
+    + destruct (lookup_struct s env) as [sdef |] eqn:Hlookup; try discriminate.
+      destruct (negb (Nat.eqb (Datatypes.length l) (struct_lifetimes sdef))) eqn:Hlts;
+        try discriminate.
+      destruct (negb (Nat.eqb (Datatypes.length l0) (struct_type_params sdef))) eqn:Hargslen;
+        try discriminate.
+      destruct (check_struct_bounds env (struct_bounds sdef) l0) as [err |] eqn:Hbounds;
+        try discriminate.
+      destruct (first_duplicate_field l1) as [dup |] eqn:Hdup; try discriminate.
+      destruct (first_unknown_field l1 (struct_fields sdef)) as [unknown |] eqn:Hunknown;
+        try discriminate.
+      destruct (first_missing_field (struct_fields sdef) l1) as [missing |] eqn:Hmissing;
+        try discriminate.
+      rewrite infer_env_fields_collect_eq in Hinfer.
+      destruct (infer_env_fields_collect fuel' env Ω n l l0 Σ l1 (struct_fields sdef))
+        as [Σfields | err] eqn:Hfields; try discriminate.
+      inversion Hinfer; subst.
+      apply negb_false_iff in Hlts. apply Nat.eqb_eq in Hlts.
+      apply negb_false_iff in Hargslen. apply Nat.eqb_eq in Hargslen.
+      eapply TES_Struct.
+      * exact Hlookup.
+      * exact Hlts.
+      * exact Hargslen.
+      * exact Hbounds.
+      * eapply infer_env_fields_collect_sound.
+        -- exact Hstruct.
+        -- exact Hfields.
+        -- intros Σ0 e0 T0 Σ1 Hexpr Hinfer0.
+           eapply IH; [exact Hexpr | exact Hinfer0].
+    + destruct (infer_place_type_sctx env Σ p) as [Told | err] eqn:Hptype; try discriminate.
+      destruct (place_path p) as [[x path] |] eqn:Hpath.
+      * destruct (sctx_lookup_mut x Σ) as [mut |] eqn:Hmut; try discriminate.
+        destruct mut; try discriminate.
+        destruct (infer_core_env_state_fuel fuel' env Ω n Σ e) as [[Tnew Σ1] | err]
+          eqn:Hnew; try discriminate.
+        destruct (ty_compatible_b Ω Tnew Told) eqn:Hcompat; try discriminate.
+        destruct (sctx_restore_path Σ1 x path) as [Σ2 | err] eqn:Hrestore; try discriminate.
+        inversion Hinfer; subst.
+        eapply TES_Replace_Path.
+        -- eapply infer_place_type_sctx_structural_sound. exact Hptype.
+        -- exact Hpath.
+        -- exact Hmut.
+        -- eapply IH; [exact Hstruct | exact Hnew].
+        -- exact Hcompat.
+        -- exact Hrestore.
+      * destruct (place_under_unique_ref_b env Σ p) eqn:Hunique; try discriminate.
+        destruct (infer_core_env_state_fuel fuel' env Ω n Σ e) as [[Tnew Σ1] | err]
+          eqn:Hnew; try discriminate.
+        destruct (ty_compatible_b Ω Tnew Told) eqn:Hcompat; try discriminate.
+        inversion Hinfer; subst.
+        eapply TES_Replace_Indirect.
+        -- eapply infer_place_type_sctx_structural_sound. exact Hptype.
+        -- exact Hpath.
+        -- apply place_under_unique_ref_b_sound. exact Hunique.
+        -- eapply IH; [exact Hstruct | exact Hnew].
+        -- exact Hcompat.
+    + destruct (infer_place_sctx env Σ p) as [Told | err] eqn:Hplace; try discriminate.
+      destruct (usage_eqb (ty_usage Told) ULinear) eqn:Hlinear; try discriminate.
+      destruct (place_path p) as [[x path] |] eqn:Hpath.
+      * destruct (sctx_lookup_mut x Σ) as [mut |] eqn:Hmut; try discriminate.
+        destruct mut; try discriminate.
+        destruct (infer_core_env_state_fuel fuel' env Ω n Σ e) as [[Tnew Σ1] | err]
+          eqn:Hnew; try discriminate.
+        destruct (ty_compatible_b Ω Tnew Told) eqn:Hcompat; try discriminate.
+        inversion Hinfer; subst.
+        eapply TES_Assign_Path.
+        -- eapply infer_place_sctx_structural_sound. exact Hplace.
+        -- intro Hu. rewrite Hu in Hlinear. simpl in Hlinear. discriminate.
+        -- exact Hpath.
+        -- exact Hmut.
+        -- eapply IH; [exact Hstruct | exact Hnew].
+        -- exact Hcompat.
+      * destruct (place_under_unique_ref_b env Σ p) eqn:Hunique; try discriminate.
+        destruct (infer_core_env_state_fuel fuel' env Ω n Σ e) as [[Tnew Σ1] | err]
+          eqn:Hnew; try discriminate.
+        destruct (ty_compatible_b Ω Tnew Told) eqn:Hcompat; try discriminate.
+        inversion Hinfer; subst.
+        eapply TES_Assign_Indirect.
+        -- eapply infer_place_sctx_structural_sound. exact Hplace.
+        -- intro Hu. rewrite Hu in Hlinear. simpl in Hlinear. discriminate.
+        -- exact Hpath.
+        -- apply place_under_unique_ref_b_sound. exact Hunique.
+        -- eapply IH; [exact Hstruct | exact Hnew].
+        -- exact Hcompat.
+    + destruct (infer_place_sctx env Σ p) as [Tp | err] eqn:Hplace; try discriminate.
+      destruct r.
+      * inversion Hinfer; subst.
+        eapply TES_BorrowShared.
+        eapply infer_place_sctx_structural_sound. exact Hplace.
+      * destruct (place_path p) as [[x path] |] eqn:Hpath.
+        -- destruct (sctx_lookup_mut x Σ) as [mut |] eqn:Hmut; try discriminate.
+           destruct mut; try discriminate.
+           inversion Hinfer; subst.
+           eapply TES_BorrowUnique.
+           ++ eapply infer_place_sctx_structural_sound. exact Hplace.
+           ++ exact Hpath.
+           ++ exact Hmut.
+        -- destruct (place_under_unique_ref_b env Σ p) eqn:Hunique; try discriminate.
+           inversion Hinfer; subst.
+           eapply TES_BorrowUnique_Indirect.
+           ++ eapply infer_place_sctx_structural_sound. exact Hplace.
+           ++ exact Hpath.
+           ++ apply place_under_unique_ref_b_sound. exact Hunique.
+    + destruct (expr_as_place e) as [p |] eqn:Hplace_expr.
+      * destruct (infer_place_sctx env Σ p) as [Tp | err] eqn:Hplace; try discriminate.
+        destruct Tp as [u c]; simpl in *.
+        destruct c; try discriminate.
+        destruct (usage_eqb (ty_usage t) UUnrestricted) eqn:Husage; try discriminate.
+        inversion Hinfer; subst.
+        eapply TES_Deref_Place.
+        -- exact Hplace_expr.
+        -- eapply infer_place_sctx_structural_sound. exact Hplace.
+        -- apply usage_eqb_true. exact Husage.
+      * destruct (infer_core_env_state_fuel fuel' env Ω n Σ e) as [[Tr Σr] | err]
+          eqn:Hr; try discriminate.
+        destruct Tr as [u c]; simpl in *.
+        destruct c; try discriminate.
+        destruct (usage_eqb (ty_usage t) UUnrestricted) eqn:Husage; try discriminate.
+        inversion Hinfer; subst.
+        eapply TES_Deref_Expr.
+        -- exact Hplace_expr.
+        -- eapply IH; [exact Hstruct | exact Hr].
+        -- apply usage_eqb_true. exact Husage.
+    + destruct (infer_core_env_state_fuel fuel' env Ω n Σ e) as [[Te Σe] | err]
+        eqn:He; try discriminate.
+      inversion Hinfer; subst.
+      eapply TES_Drop. eapply IH; [exact Hstruct | exact He].
+    + repeat rewrite andb_true_iff in Hstruct.
+      destruct Hstruct as [[Hstruct1 Hstruct2] Hstruct3].
+      destruct (infer_core_env_state_fuel fuel' env Ω n Σ e1) as [[Tcond Σ1] | err1]
+        eqn:He1; try discriminate.
+      destruct (ty_core_eqb (ty_core Tcond) TBooleans) eqn:Hbool; try discriminate.
+      destruct (infer_core_env_state_fuel fuel' env Ω n Σ1 e2) as [[T2 Σ2] | err2]
+        eqn:He2; try discriminate.
+      destruct (infer_core_env_state_fuel fuel' env Ω n Σ1 e3) as [[T3 Σ3] | err3]
+        eqn:He3; try discriminate.
+      destruct (ty_core_eqb (ty_core T2) (ty_core T3)) eqn:Hcore; try discriminate.
+      destruct (ctx_merge (ctx_of_sctx Σ2) (ctx_of_sctx Σ3)) as [Γ4 |] eqn:Hmerge;
+        try discriminate.
+      inversion Hinfer; subst.
+      eapply TES_If.
+      * eapply IH; [exact Hstruct1 | exact He1].
+      * apply ty_core_eqb_true. exact Hbool.
+      * eapply IH; [exact Hstruct2 | exact He2].
+      * eapply IH; [exact Hstruct3 | exact He3].
       * apply ty_core_eqb_true. exact Hcore.
       * exact Hmerge.
 Qed.
